<?xml version="1.0"?>
<rdf:RDF xmlns="https://nvd.nist.gov/Products/CPE#"
     xml:base="https://nvd.nist.gov/Products/CPE"
     xmlns:rdf="http://www.w3.org/1999/02/22-rdf-syntax-ns#"
     xmlns:owl="http://www.w3.org/2002/07/owl#"
     xmlns:xml="http://www.w3.org/XML/1998/namespace"
     xmlns:xsd="http://www.w3.org/2001/XMLSchema#"
     xmlns:cpe="https://nvd.nist.gov/Products/CPE"
     xmlns:rdfs="http://www.w3.org/2000/01/rdf-schema#">
    <owl:Ontology rdf:about="https://nvd.nist.gov/Products/CPE">
        <rdfs:label xml:lang="en">Common Platform Enumeration Ontology (CPE)</rdfs:label>
        <rdfs:comment xml:lang="en">CPE is a structured naming scheme for information technology systems, software, and packages. Based upon the generic syntax for Uniform Resource Identifiers (URI), CPE includes a formal name format, a method for checking names against a system, and a description format for binding text and tests to a name.</rdfs:comment>
        <rdfs:comment xml:lang="en">Created by Vasileios Mavroeidis for Oslo Analytics Project funded by the Reasearch Council of Norway. This ontology and its expansion is used as a sub-component of semanTIo (cyber threat intelligence ontology).

semanTIo URL:</rdfs:comment>
    </owl:Ontology>
    


    <!-- 
    ///////////////////////////////////////////////////////////////////////////////////////
    //
    // Data properties
    //
    ///////////////////////////////////////////////////////////////////////////////////////
     -->

    


    <!-- https://nvd.nist.gov/Products/CPE#hasCpe23 -->

    <owl:DatatypeProperty rdf:about="https://nvd.nist.gov/Products/CPE#hasCpe23">
        <rdfs:range rdf:resource="http://www.w3.org/2001/XMLSchema#string"/>
    </owl:DatatypeProperty>
    


    <!-- https://nvd.nist.gov/Products/CPE#hasCpeReference -->

    <owl:DatatypeProperty rdf:about="https://nvd.nist.gov/Products/CPE#hasCpeReference">
        <rdfs:range rdf:resource="http://www.w3.org/2001/XMLSchema#anyURI"/>
    </owl:DatatypeProperty>
    


    <!-- https://nvd.nist.gov/Products/CPE#hasCpeTitle -->

    <owl:DatatypeProperty rdf:about="https://nvd.nist.gov/Products/CPE#hasCpeTitle">
        <rdfs:range rdf:resource="http://www.w3.org/2001/XMLSchema#string"/>
    </owl:DatatypeProperty>
    


    <!-- 
    ///////////////////////////////////////////////////////////////////////////////////////
    //
    // Classes
    //
    ///////////////////////////////////////////////////////////////////////////////////////
     -->

    


    <!-- https://nvd.nist.gov/Products/CPE#Cpe -->

    <owl:Class rdf:about="https://nvd.nist.gov/Products/CPE#Cpe">
        <owl:equivalentClass>
            <owl:Class>
                <owl:intersectionOf rdf:parseType="Collection">
                    <owl:Restriction>
                        <owl:onProperty rdf:resource="https://nvd.nist.gov/Products/CPE#hasCpe23"/>
                        <owl:someValuesFrom rdf:resource="http://www.w3.org/2001/XMLSchema#string"/>
                    </owl:Restriction>
                    <owl:Restriction>
                        <owl:onProperty rdf:resource="https://nvd.nist.gov/Products/CPE#hasCpeTitle"/>
                        <owl:someValuesFrom rdf:resource="http://www.w3.org/2001/XMLSchema#string"/>
                    </owl:Restriction>
                    <owl:Restriction>
                        <owl:onProperty rdf:resource="https://nvd.nist.gov/Products/CPE#hasCpeReference"/>
                        <owl:minQualifiedCardinality rdf:datatype="http://www.w3.org/2001/XMLSchema#nonNegativeInteger">0</owl:minQualifiedCardinality>
                        <owl:onDataRange rdf:resource="http://www.w3.org/2001/XMLSchema#anyURI"/>
                    </owl:Restriction>
                </owl:intersectionOf>
            </owl:Class>
        </owl:equivalentClass>
        <rdfs:comment xml:lang="en">CPE is a structured naming scheme for information technology systems, software, and packages. Based upon the generic syntax for Uniform Resource Identifiers (URI), CPE includes a formal name format, a method for checking names against a system, and a description format for binding text and tests to a name.</rdfs:comment>
        <rdfs:comment xml:lang="en">The CPE dictionary includes:

cpe name = Cpe
title = hasTitle
references = hasCpeReference
cpe-23 = hasCpe23</rdfs:comment>
    </owl:Class>
</rdf:RDF>



<!-- Generated by the OWL API (version 4.2.8.20170104-2310) https://github.com/owlcs/owlapi -->

